$F=\left( \begin{array}{ccc} -1 & +1 & 0 \\ 0 & 0 & -1 \\ +1 & 0 & -1 \end{array} \right) $
$F=\left( \begin{array}{ccc} 0 & +1 & 0 \\ 0 & +1 & -1 \\ +1 & -1 & -1 \end{array} \right) $
$F=\left( \begin{array}{ccc} +1 & 0 & 0 \\ 0 & 0 & +1 \\ -1 & -1 & -1 \end{array} \right) $
$F=\left( \begin{array}{ccc} +1 & +1 & +1 \\ -1 & 0 & -1 \\ 0 & 0 & -1 \end{array} \right) $
$F=\left( \begin{array}{ccc} +1 & 0 & 0  \\ 0 & +1 & +1 \\ +1 & 0 & 0 \end{array} \right) $
$F=\left( \begin{array}{ccc} 0 & 0 & -1 \\ -1 & -1 & -1 \\ 0 & +1 & 0 \end{array} \right) $
$F=\left( \begin{array}{ccc} -1 & -1 & +1 \\ +1 & 0 & 0 \\ 0 & +1 & +1 \end{array} \right) $
$F=\left( \begin{array}{ccc} +1 & +1 & +1 \\ -1 & +1 & -1 \\ +1 & -1 & 0 \end{array} \right) $
